modified Oracle contract so it could send attestation to an arbitrary recipient

Oracle2/Oracle2.fst
@@ -12,9 +12,16 @@ module Sha3 = Zen.Hash.Sha3
 module TX = Zen.TxSkeleton
 module W = Zen.Wallet
 
-type args =
+
+
+type commitData =
     { commit       : hash
     ; oraclePubKey : publicKey
+    }
+
+type attestData =
+    { commitData : commitData
+    ; recipient  : lock
     }
 
 type assets =
@@ -25,133 +32,294 @@ type assets =
 // compressed public key
 type cpk = byte ** hash
 
-let parseArgs (pk : option publicKey) (msg: option data): result args `cost` 167 = // 37
-    let open OT in
-    match msg with
-    | Some (Collection (Dict dict)) -> begin
-        let! commit = Dict.tryFind "Commit" dict in // 64
-        let! oraclePubKey =
-          begin match pk with
-          | None ->
-              Dict.tryFind "OraclePubKey" dict // 64
-              >>= Zen.Data.tryPublicKey // 2
-          | Some pk ->
-              pk
-              |> incSome 66
-          end
-        in match commit, oraclePubKey with
-        | Some (Hash commit), Some oraclePubKey ->
-            RT.ok ({ commit=commit;
-                     oraclePubKey=oraclePubKey })
-        | _, Some _ ->
-            RT.failw "Could not parse Commit"
-        | Some (Hash _), None ->
-            RT.failw "Could not parse OraclePubKey"
-        | _, None ->
-            RT.failw "Could not parse Commit & OraclePubKey"
-        end
-    | _ -> RT.autoFailw "MessageBody must be a dictionary."
 
-// compress a public key
-let compress (pk:publicKey): cpk `cost` 305 =  // 13
+
+(*
+-------------------------------------------------------------------------------
+========== COMPRESSED PUBLIC KEY ==============================================
+-------------------------------------------------------------------------------
+*)
+
+val compress : publicKey -> cpk `cost` 305
+let compress pk = // 13
     let open FStar.UInt8 in
     let parity = (Zen.Array.item 32 pk %^ 2uy) +^ 2uy in
-    let aux (i:nat{i < 32}): byte `cost` 5 =
-        ret (Zen.Array.item (31-i) pk) in
+    let aux (i:nat{i < 32}): byte `cost` 5 = ret (Zen.Array.item (31-i) pk) in
     let! x = Zen.Array.init_pure 32 aux in // 292
-    ret (parity, x)
+    ret (parity , x)
 
-let updateCPK ((parity, h):cpk) (s:Sha3.t): Sha3.t `cost` 203 = // 5
-    Sha3.updateByte parity s
+val updateCPK : cpk -> Sha3.t -> Sha3.t `cost` 205
+let updateCPK (parity , h) s = // 7
+    ret s
+    >>= Sha3.updateByte parity
     >>= Sha3.updateHash h
 
-// hash a compressed publicKey
-let hashCPK (cpk:cpk): hash `cost` 227 = // 4
-    updateCPK cpk Sha3.empty // 203
+val hashCPK : cpk -> hash `cost` 231
+let hashCPK cpk = // 6
+    ret Sha3.empty
+    >>= updateCPK cpk // 205
     >>= Sha3.finalize // 20
 
-let hashArgs (args:args): hash `cost` 732 = // 12
-    let! cpk = compress args.oraclePubKey in // 305
-    Sha3.updateHash args.commit Sha3.empty // 192
-    >>= updateCPK cpk // 203
-    >>= Sha3.finalize // 20
 
-val mkAssets: contractId -> args:args -> assets `cost` 962
-let mkAssets (v, h) args = // 18
-    let! argsHash = hashArgs args in // 732
-    let! arsgHash2 = Sha3.updateHash argsHash Sha3.empty // 192
-                     >>= Sha3.finalize in // 20
-    ret ({ commitment=v,h,argsHash; attestation=v,h,arsgHash2 })
 
-//
-// Making a commitment
-//
+(*
+-------------------------------------------------------------------------------
+========== DATA PARSING =======================================================
+-------------------------------------------------------------------------------
+*)
 
-val commit: txSkeleton -> contractId -> publicKey -> args -> CR.t `cost` 1107
-let commit tx cid senderPK args = // 14
-    let! ({commitment=commitment}) = mkAssets cid args in // 962
-    // mint the commitment token
-    TX.mint 1UL commitment tx // 64
-    // lock the commitment token to the contract
+val parseCommitData : publicKey -> option data -> commitData `RT.t` 81
+let parseCommitData sender msgBody = // 17
+    begin match msgBody with
+    | Some (Collection (Dict dict)) ->
+        let! commit = Dict.tryFind "Commit" dict in // 64
+        begin match commit with
+        | Some (Hash commit) ->
+            { commit       = commit
+            ; oraclePubKey = sender
+            } |> RT.ok
+        | _ ->
+            RT.failw "Could not parse Commit"
+        end
+    | _ ->
+        RT.autoFailw "MessageBody must be a dictionary."
+    end
+
+val senderToLock : sender -> lock `OT.t` 551
+let senderToLock sender = // 15
+    begin match sender with
+    | PK pk ->
+        let! pkHash =
+            ret pk
+            >>= compress // 305
+            >>= hashCPK  // 231
+        in ret (Some (PKLock pkHash))
+    | Contract cid ->
+        Some (ContractLock cid)
+        |> incRet 536
+    | Anonymous ->
+        None
+        |> incRet 536
+    end
+
+val parseAttestData : sender -> option data -> attestData `RT.t` 813
+let parseAttestData sender msgBody = // 70
+    begin match msgBody with
+    | Some (Collection (Dict dict)) ->
+        let! commit       = Dict.tryFind "Commit"       dict in // 64
+        let! oraclePubKey = Dict.tryFind "OraclePubKey" dict in // 64
+        let! recipient    = Dict.tryFind "Recipient"    dict in // 64
+        let! senderLock   = senderToLock sender              in // 551
+        begin match commit , oraclePubKey , recipient with
+        | Some (Hash commit) , Some (PublicKey pk) , Some (Lock recip) ->
+            { commitData =
+                { commit       = commit
+                ; oraclePubKey = pk
+                }
+            ; recipient = recip
+            } |> RT.ok
+        | Some (Hash commit) , Some (PublicKey pk) , None ->
+            begin match senderLock with
+            | Some lock ->
+                { commitData =
+                    { commit       = commit
+                    ; oraclePubKey = pk
+                    }
+                ; recipient = lock
+                } |> RT.ok
+            | None ->
+                RT.failw "Unspecified recipient"
+            end
+        | Some (Hash _) , Some (PublicKey _) , Some _ ->
+            RT.failw "Recipient must be a lock"
+        | _ , Some _ , _ ->
+            RT.failw "OraclePubKey must be a public key"
+        | _ , None , _ ->
+            RT.failw "Couldn't find OraclePubKey in message body"
+        | Some _ , _ , _ ->
+            RT.failw "Commit must be an hash"
+        | None , _ , _ ->
+            RT.failw "Couldn't find Commit in message body"
+        end
+    | _ -> RT.autoFailw "MessageBody must be a dictionary."
+    end
+
+
+
+(*
+-------------------------------------------------------------------------------
+========== TOKENIZATION =======================================================
+-------------------------------------------------------------------------------
+*)
+
+val hashCommitData : commitData -> hash `cost` 736
+let hashCommitData data = // 14
+    let! cpk = compress data.oraclePubKey in // 305
+    ret Sha3.empty
+    >>= Sha3.updateHash data.commit // 192
+    >>= updateCPK cpk               // 205
+    >>= Sha3.finalize               // 20
+
+val mkAssets : contractId -> commitData -> assets `cost` 968
+let mkAssets (v, h) data = // 20
+    let! dataHash =
+        hashCommitData data in // 736
+    let! dataHash2 =
+        ret Sha3.empty
+        >>= Sha3.updateHash dataHash // 192
+        >>= Sha3.finalize in         // 20
+    ret ({ commitment=v,h,dataHash; attestation=v,h,dataHash2 })
+
+
+
+(*
+-------------------------------------------------------------------------------
+========== COMMAND: Commit ====================================================
+-------------------------------------------------------------------------------
+*)
+
+val dataCommit :
+    txSkeleton
+    -> contractId
+    -> commitData
+    -> txSkeleton `cost` 1110
+let dataCommit txSkel cid args = // 14
+    let! ({commitment = commitment}) = mkAssets cid args in // 968
+    ret txSkel
+    >>= TX.mint 1UL commitment               // 64
     >>= TX.lockToContract commitment 1UL cid // 64
-    // return the tx
-    >>= CR.ofTxSkel // 3
 
-//
-// Attesting to a commitment
-//
-
-let lockToPK (s:spend) (pk:publicKey) (tx:txSkeleton): txSkeleton `cost` 608 = // 12
-    let! pkHash = compress pk >>= hashCPK in // 305 + 227
-    TX.lockToAddress s.asset s.amount (PKLock pkHash) tx // 64
-
-// The attestation transaction, minus contract wallet inputs
-let attestTx tx cid senderPK assets: txSkeleton `cost` 891 = // 27
-    // destroy the attestation token
-    TX.destroy 1UL assets.commitment tx // 64
-    // mint the new commitment and attestation tokens
-    >>= TX.mint 1UL assets.commitment // 64
-    >>= TX.mint 1UL assets.attestation // 64
-    // lock the attestation token to the user
-    >>= lockToPK ({asset=assets.attestation; amount=1UL}) senderPK // 608
-    // lock the commitment token to the contract
-    >>= TX.lockToContract assets.commitment 1UL cid // 64
-
-let attest tx cid senderPK w (args:args) : contractResult `cost` (962 + (891 + (Zen.Wallet.size w * 128 + 192) + 3) + 18) = // 18
-    let! assets = mkAssets cid args in // 962
-    // the tx, minus contract wallet inputs
-    attestTx tx cid senderPK assets // 891
-    // add a commitment token from the contract wallet
-    >>= TX.fromWallet assets.commitment 1UL cid w // W.size w * 128 + 192
-    // return the tx
-    >>= CR.ofOptionTxSkel "Could not spend from wallet" // 3
-
-//
-// Exports
-//
-
-let main tx _ cid command sender msg w _ = // 21
+val commit :
+  contractId
+  -> sender
+  -> option data
+  -> txSkeleton
+  -> CR.t `cost` 1210
+let commit cid sender msgBody txSkel = // 16
     let open RT in
-    match command, sender with
-    | "Commit", PK pk ->
-        parseArgs (Some pk) msg // 167
-        >>= commit tx cid pk // 1107
-        <: CR.t `cost` begin match command, sender with
-                       | "Commit", PK _ -> 1274
-                       | "Attest", PK _ -> 167 + (962 + (891 + (Zen.Wallet.size w * 128 + 192) + 3) + 18)
-                       | _ -> 0 end
-    | "Attest", PK pk ->
-        parseArgs None msg // 167
-        >>= attest tx cid pk w // (962 + (891 + (Zen.Wallet.size w * 128 + 192) + 3) + 18)
-    | _, PK pk ->
-        failw "Command not recognized"
-    | _, _ ->
-        failw "Sender must be a public key"
+    let! tx =
+        begin match sender with
+        | PK pk ->
+            ret msgBody
+            >>= parseCommitData pk                  // 81
+            >>= (liftCost << dataCommit txSkel cid) // 1110
+        | _ ->
+            "Sender must be a public key"
+            |> RT.incFailw 1191
+        end
+    in CR.ofResultTxSkel tx // 3
 
-let cf _ _ command sender _ w _ : nat `cost` 27 = // 27
-    ret ((match command, sender with
-          | "Commit", Zen.Types.Main.PK _ -> 1274
-          | "Attest", Zen.Types.Main.PK _ ->
-            167 + (962 + (891 + (Zen.Wallet.size w * 128 + 192) + 3) + 18)
-          | _ -> 0)
-        + 21)
+
+
+(*
+-------------------------------------------------------------------------------
+========== COMMAND: Attest ====================================================
+-------------------------------------------------------------------------------
+*)
+
+val attestTx :
+    assets
+    -> contractId
+    -> (w : wallet)
+    -> lock
+    -> txSkeleton
+    -> txSkeleton `OT.t` (128 + (W.size w * 128 + 192) + 64 + 31)
+let attestTx assets cid (w : wallet) (recipient : lock) txSkel = // 31
+    let open OT in
+    ret txSkel
+    >>= (liftCost << TX.mint 1UL assets.attestation) // 64
+    >>= (liftCost << TX.lockToAddress assets.attestation 1UL recipient) // 64
+    >>= TX.fromWallet assets.commitment 1UL cid w // W.size w * 128 + 192
+    >>= (liftCost << TX.lockToContract assets.commitment 1UL cid) // 64
+
+val dataAttest' :
+    contractId
+    -> (w : wallet)
+    -> txSkeleton
+    -> attestData
+    -> txSkeleton `RT.t` (968 + (0 + (128 + (W.size w * 128 + 192) + 64 + 31) + 0) + 16)
+let dataAttest' cid w txSkel args = // 16
+    let! assets = mkAssets cid args.commitData in // 968
+    ret txSkel
+    >>= attestTx assets cid w args.recipient
+    >>= RT.ofOption "Could not spend from wallet"
+
+val dataAttest :
+    contractId
+    -> (w : wallet)
+    -> txSkeleton
+    -> attestData
+    -> txSkeleton `RT.t` (W.size w * 128 + 1405)
+let dataAttest cid w txSkel args = // 16
+    dataAttest' cid w txSkel args
+    |> (fun x -> x <: txSkeleton `RT.t` (W.size w * 128 + 1399))
+
+val attest :
+    contractId ->
+    (w : wallet) ->
+    sender ->
+    option data ->
+    txSkeleton ->
+    CR.t `cost` (W.size w * 128 + 2231)
+let attest cid w sender msgBody txSkel = // 10
+    let open RT in
+    let! tx =
+        parseAttestData sender msgBody // 813
+        >>= dataAttest cid w txSkel // W.size w * 128 + 1405
+    in CR.ofResultTxSkel tx // 3
+
+
+
+(*
+-------------------------------------------------------------------------------
+========== MAIN ===============================================================
+-------------------------------------------------------------------------------
+*)
+
+val main :
+       txSkel  : txSkeleton
+    -> context : context
+    -> cid     : contractId
+    -> command : string
+    -> sender  : sender
+    -> msgBody : option data
+    -> w       : wallet
+    -> state   : option data
+    -> CR.t `cost`
+        begin match command with
+        | "Commit" -> 1218
+        | "Attest" -> W.size w * 128 + 2239
+        | _        -> 8
+        end
+let main txSkel _ cid command sender msgBody w _ = // 8
+    begin match command with
+    | "Commit" ->
+        commit cid sender msgBody txSkel // 1210
+        <: CR.t `cost`
+            begin match command with
+            | "Commit" -> 1210
+            | "Attest" -> W.size w * 128 + 2231
+            | _        -> 0
+            end
+    | "Attest" ->
+        attest cid w sender msgBody txSkel // W.size w * 128 + 2231
+    | _ ->
+        RT.failw "Command not recognized"
+    end
+
+val cf :
+       txSkel     : txSkeleton
+    -> context    : context
+    -> command    : string
+    -> sender     : sender
+    -> messageBody: option data
+    -> w          : wallet
+    -> state      : option data
+    -> nat `cost` 10
+let cf _ _ command _ _ w _ = // 10
+    begin match command with
+    | "Commit" -> 1218
+    | "Attest" -> W.size w * 128 + 2239
+    | _        -> 8
+    end
+    |> ret
